AwsCryptographicMaterialProviders/runtimes/java/src/main/smithy-generated/software/amazon/cryptography/materialProviders/model/CreateExpectedEncryptionContextCMMInput.java
@@ -1,0 +1,112 @@
+// Copyright Amazon.com Inc. or its affiliates. All Rights Reserved.
+// SPDX-License-Identifier: Apache-2.0
+// Do not modify this file. This file is machine generated, and any changes to it will be overwritten.
+package software.amazon.cryptography.materialProviders.model;
+
+import java.util.List;
+import java.util.Objects;
+import software.amazon.cryptography.materialProviders.CryptographicMaterialsManager;
+import software.amazon.cryptography.materialProviders.ICryptographicMaterialsManager;
+import software.amazon.cryptography.materialProviders.IKeyring;
+import software.amazon.cryptography.materialProviders.Keyring;
+
+public class CreateExpectedEncryptionContextCMMInput {
+  private final CryptographicMaterialsManager underlyingCMM;
+
+  private final Keyring keyring;
+
+  private final List<String> requiredEncryptionContextKeys;
+
+  protected CreateExpectedEncryptionContextCMMInput(BuilderImpl builder) {
+    this.underlyingCMM = builder.underlyingCMM();
+    this.keyring = builder.keyring();
+    this.requiredEncryptionContextKeys = builder.requiredEncryptionContextKeys();
+  }
+
+  public CryptographicMaterialsManager underlyingCMM() {
+    return this.underlyingCMM;
+  }
+
+  public Keyring keyring() {
+    return this.keyring;
+  }
+
+  public List<String> requiredEncryptionContextKeys() {
+    return this.requiredEncryptionContextKeys;
+  }
+
+  public Builder toBuilder() {
+    return new BuilderImpl(this);
+  }
+
+  public static Builder builder() {
+    return new BuilderImpl();
+  }
+
+  public interface Builder {
+    Builder underlyingCMM(ICryptographicMaterialsManager underlyingCMM);
+
+    CryptographicMaterialsManager underlyingCMM();
+
+    Builder keyring(IKeyring keyring);
+
+    Keyring keyring();
+
+    Builder requiredEncryptionContextKeys(List<String> requiredEncryptionContextKeys);
+
+    List<String> requiredEncryptionContextKeys();
+
+    CreateExpectedEncryptionContextCMMInput build();
+  }
+
+  static class BuilderImpl implements Builder {
+    protected CryptographicMaterialsManager underlyingCMM;
+
+    protected Keyring keyring;
+
+    protected List<String> requiredEncryptionContextKeys;
+
+    protected BuilderImpl() {
+    }
+
+    protected BuilderImpl(CreateExpectedEncryptionContextCMMInput model) {
+      this.underlyingCMM = model.underlyingCMM();
+      this.keyring = model.keyring();
+      this.requiredEncryptionContextKeys = model.requiredEncryptionContextKeys();
+    }
+
+    public Builder underlyingCMM(ICryptographicMaterialsManager underlyingCMM) {
+      this.underlyingCMM = CryptographicMaterialsManager.wrap(underlyingCMM);
+      return this;
+    }
+
+    public CryptographicMaterialsManager underlyingCMM() {
+      return this.underlyingCMM;
+    }
+
+    public Builder keyring(IKeyring keyring) {
+      this.keyring = Keyring.wrap(keyring);
+      return this;
+    }
+
+    public Keyring keyring() {
+      return this.keyring;
+    }
+
+    public Builder requiredEncryptionContextKeys(List<String> requiredEncryptionContextKeys) {
+      this.requiredEncryptionContextKeys = requiredEncryptionContextKeys;
+      return this;
+    }
+
+    public List<String> requiredEncryptionContextKeys() {
+      return this.requiredEncryptionContextKeys;
+    }
+
+    public CreateExpectedEncryptionContextCMMInput build() {
+      if (Objects.isNull(this.requiredEncryptionContextKeys()))  {
+        throw new IllegalArgumentException("Missing value for required field `requiredEncryptionContextKeys`");
+      }
+      return new CreateExpectedEncryptionContextCMMInput(this);
+    }
+  }
+}
