AwsCryptographicMaterialProviders/runtimes/net/Generated/CreateExpectedEncryptionContextCMMInput.cs
@@ -1,0 +1,46 @@
+// Copyright Amazon.com Inc. or its affiliates. All Rights Reserved.
+// SPDX-License-Identifier: Apache-2.0
+// Do not modify this file. This file is machine generated, and any changes to it will be overwritten.
+using System;
+using AWS.Cryptography.MaterialProviders;
+namespace AWS.Cryptography.MaterialProviders
+{
+  public class CreateExpectedEncryptionContextCMMInput
+  {
+    private AWS.Cryptography.MaterialProviders.ICryptographicMaterialsManager _underlyingCMM;
+    private AWS.Cryptography.MaterialProviders.IKeyring _keyring;
+    private System.Collections.Generic.List<string> _requiredEncryptionContextKeys;
+    public AWS.Cryptography.MaterialProviders.ICryptographicMaterialsManager UnderlyingCMM
+    {
+      get { return this._underlyingCMM; }
+      set { this._underlyingCMM = value; }
+    }
+    public bool IsSetUnderlyingCMM()
+    {
+      return this._underlyingCMM != null;
+    }
+    public AWS.Cryptography.MaterialProviders.IKeyring Keyring
+    {
+      get { return this._keyring; }
+      set { this._keyring = value; }
+    }
+    public bool IsSetKeyring()
+    {
+      return this._keyring != null;
+    }
+    public System.Collections.Generic.List<string> RequiredEncryptionContextKeys
+    {
+      get { return this._requiredEncryptionContextKeys; }
+      set { this._requiredEncryptionContextKeys = value; }
+    }
+    public bool IsSetRequiredEncryptionContextKeys()
+    {
+      return this._requiredEncryptionContextKeys != null;
+    }
+    public void Validate()
+    {
+      if (!IsSetRequiredEncryptionContextKeys()) throw new System.ArgumentException("Missing value for required property 'RequiredEncryptionContextKeys'");
+
+    }
+  }
+}
