AwsCryptographicMaterialProviders/runtimes/net/Generated/TypeConversion.cs
@@ -294,6 +294,26 @@ namespace AWS.Cryptography.MaterialProviders
 
       return new Dafny.Aws.Cryptography.MaterialProviders.Types.CreateDefaultCryptographicMaterialsManagerInput(ToDafny_N3_aws__N12_cryptography__N17_materialProviders__S47_CreateDefaultCryptographicMaterialsManagerInput__M7_keyring(value.Keyring));
     }
+    internal static AWS.Cryptography.MaterialProviders.CreateExpectedEncryptionContextCMMInput FromDafny_N3_aws__N12_cryptography__N17_materialProviders__S39_CreateExpectedEncryptionContextCMMInput(Dafny.Aws.Cryptography.MaterialProviders.Types._ICreateExpectedEncryptionContextCMMInput value)
+    {
+      Dafny.Aws.Cryptography.MaterialProviders.Types.CreateExpectedEncryptionContextCMMInput concrete = (Dafny.Aws.Cryptography.MaterialProviders.Types.CreateExpectedEncryptionContextCMMInput)value; AWS.Cryptography.MaterialProviders.CreateExpectedEncryptionContextCMMInput converted = new AWS.Cryptography.MaterialProviders.CreateExpectedEncryptionContextCMMInput(); if (concrete._underlyingCMM.is_Some) converted.UnderlyingCMM = (AWS.Cryptography.MaterialProviders.ICryptographicMaterialsManager)FromDafny_N3_aws__N12_cryptography__N17_materialProviders__S39_CreateExpectedEncryptionContextCMMInput__M13_underlyingCMM(concrete._underlyingCMM);
+      if (concrete._keyring.is_Some) converted.Keyring = (AWS.Cryptography.MaterialProviders.IKeyring)FromDafny_N3_aws__N12_cryptography__N17_materialProviders__S39_CreateExpectedEncryptionContextCMMInput__M7_keyring(concrete._keyring);
+      converted.RequiredEncryptionContextKeys = (System.Collections.Generic.List<string>)FromDafny_N3_aws__N12_cryptography__N17_materialProviders__S39_CreateExpectedEncryptionContextCMMInput__M29_requiredEncryptionContextKeys(concrete._requiredEncryptionContextKeys); return converted;
+    }
+    internal static Dafny.Aws.Cryptography.MaterialProviders.Types._ICreateExpectedEncryptionContextCMMInput ToDafny_N3_aws__N12_cryptography__N17_materialProviders__S39_CreateExpectedEncryptionContextCMMInput(AWS.Cryptography.MaterialProviders.CreateExpectedEncryptionContextCMMInput value)
+    {
+      AWS.Cryptography.MaterialProviders.ICryptographicMaterialsManager var_underlyingCMM = value.IsSetUnderlyingCMM() ? value.UnderlyingCMM : (AWS.Cryptography.MaterialProviders.ICryptographicMaterialsManager)null;
+      AWS.Cryptography.MaterialProviders.IKeyring var_keyring = value.IsSetKeyring() ? value.Keyring : (AWS.Cryptography.MaterialProviders.IKeyring)null;
+      return new Dafny.Aws.Cryptography.MaterialProviders.Types.CreateExpectedEncryptionContextCMMInput(ToDafny_N3_aws__N12_cryptography__N17_materialProviders__S39_CreateExpectedEncryptionContextCMMInput__M13_underlyingCMM(var_underlyingCMM), ToDafny_N3_aws__N12_cryptography__N17_materialProviders__S39_CreateExpectedEncryptionContextCMMInput__M7_keyring(var_keyring), ToDafny_N3_aws__N12_cryptography__N17_materialProviders__S39_CreateExpectedEncryptionContextCMMInput__M29_requiredEncryptionContextKeys(value.RequiredEncryptionContextKeys));
+    }
+    internal static AWS.Cryptography.MaterialProviders.ICryptographicMaterialsManager FromDafny_N3_aws__N12_cryptography__N17_materialProviders__S40_CreateExpectedEncryptionContextCMMOutput(Dafny.Aws.Cryptography.MaterialProviders.Types.ICryptographicMaterialsManager value)
+    {
+      return FromDafny_N3_aws__N12_cryptography__N17_materialProviders__S40_CreateExpectedEncryptionContextCMMOutput__M16_materialsManager(value);
+    }
+    internal static Dafny.Aws.Cryptography.MaterialProviders.Types.ICryptographicMaterialsManager ToDafny_N3_aws__N12_cryptography__N17_materialProviders__S40_CreateExpectedEncryptionContextCMMOutput(AWS.Cryptography.MaterialProviders.ICryptographicMaterialsManager value)
+    {
+      return ToDafny_N3_aws__N12_cryptography__N17_materialProviders__S40_CreateExpectedEncryptionContextCMMOutput__M16_materialsManager(value);
+    }
     internal static AWS.Cryptography.MaterialProviders.IKeyring FromDafny_N3_aws__N12_cryptography__N17_materialProviders__S19_CreateKeyringOutput(Dafny.Aws.Cryptography.MaterialProviders.Types.IKeyring value)
     {
       return FromDafny_N3_aws__N12_cryptography__N17_materialProviders__S19_CreateKeyringOutput__M7_keyring(value);
@@ -1478,6 +1498,38 @@ namespace AWS.Cryptography.MaterialProviders
     {
       return ToDafny_N3_aws__N12_cryptography__N17_materialProviders__S16_KeyringReference(value);
     }
+    internal static AWS.Cryptography.MaterialProviders.ICryptographicMaterialsManager FromDafny_N3_aws__N12_cryptography__N17_materialProviders__S39_CreateExpectedEncryptionContextCMMInput__M13_underlyingCMM(Wrappers_Compile._IOption<Dafny.Aws.Cryptography.MaterialProviders.Types.ICryptographicMaterialsManager> value)
+    {
+      return value.is_None ? (AWS.Cryptography.MaterialProviders.ICryptographicMaterialsManager)null : FromDafny_N3_aws__N12_cryptography__N17_materialProviders__S38_CryptographicMaterialsManagerReference(value.Extract());
+    }
+    internal static Wrappers_Compile._IOption<Dafny.Aws.Cryptography.MaterialProviders.Types.ICryptographicMaterialsManager> ToDafny_N3_aws__N12_cryptography__N17_materialProviders__S39_CreateExpectedEncryptionContextCMMInput__M13_underlyingCMM(AWS.Cryptography.MaterialProviders.ICryptographicMaterialsManager value)
+    {
+      return value == null ? Wrappers_Compile.Option<Dafny.Aws.Cryptography.MaterialProviders.Types.ICryptographicMaterialsManager>.create_None() : Wrappers_Compile.Option<Dafny.Aws.Cryptography.MaterialProviders.Types.ICryptographicMaterialsManager>.create_Some(ToDafny_N3_aws__N12_cryptography__N17_materialProviders__S38_CryptographicMaterialsManagerReference((AWS.Cryptography.MaterialProviders.ICryptographicMaterialsManager)value));
+    }
+    internal static AWS.Cryptography.MaterialProviders.IKeyring FromDafny_N3_aws__N12_cryptography__N17_materialProviders__S39_CreateExpectedEncryptionContextCMMInput__M7_keyring(Wrappers_Compile._IOption<Dafny.Aws.Cryptography.MaterialProviders.Types.IKeyring> value)
+    {
+      return value.is_None ? (AWS.Cryptography.MaterialProviders.IKeyring)null : FromDafny_N3_aws__N12_cryptography__N17_materialProviders__S16_KeyringReference(value.Extract());
+    }
+    internal static Wrappers_Compile._IOption<Dafny.Aws.Cryptography.MaterialProviders.Types.IKeyring> ToDafny_N3_aws__N12_cryptography__N17_materialProviders__S39_CreateExpectedEncryptionContextCMMInput__M7_keyring(AWS.Cryptography.MaterialProviders.IKeyring value)
+    {
+      return value == null ? Wrappers_Compile.Option<Dafny.Aws.Cryptography.MaterialProviders.Types.IKeyring>.create_None() : Wrappers_Compile.Option<Dafny.Aws.Cryptography.MaterialProviders.Types.IKeyring>.create_Some(ToDafny_N3_aws__N12_cryptography__N17_materialProviders__S16_KeyringReference((AWS.Cryptography.MaterialProviders.IKeyring)value));
+    }
+    internal static System.Collections.Generic.List<string> FromDafny_N3_aws__N12_cryptography__N17_materialProviders__S39_CreateExpectedEncryptionContextCMMInput__M29_requiredEncryptionContextKeys(Dafny.ISequence<Dafny.ISequence<byte>> value)
+    {
+      return FromDafny_N3_aws__N12_cryptography__N17_materialProviders__S21_EncryptionContextKeys(value);
+    }
+    internal static Dafny.ISequence<Dafny.ISequence<byte>> ToDafny_N3_aws__N12_cryptography__N17_materialProviders__S39_CreateExpectedEncryptionContextCMMInput__M29_requiredEncryptionContextKeys(System.Collections.Generic.List<string> value)
+    {
+      return ToDafny_N3_aws__N12_cryptography__N17_materialProviders__S21_EncryptionContextKeys(value);
+    }
+    internal static AWS.Cryptography.MaterialProviders.ICryptographicMaterialsManager FromDafny_N3_aws__N12_cryptography__N17_materialProviders__S40_CreateExpectedEncryptionContextCMMOutput__M16_materialsManager(Dafny.Aws.Cryptography.MaterialProviders.Types.ICryptographicMaterialsManager value)
+    {
+      return FromDafny_N3_aws__N12_cryptography__N17_materialProviders__S38_CryptographicMaterialsManagerReference(value);
+    }
+    internal static Dafny.Aws.Cryptography.MaterialProviders.Types.ICryptographicMaterialsManager ToDafny_N3_aws__N12_cryptography__N17_materialProviders__S40_CreateExpectedEncryptionContextCMMOutput__M16_materialsManager(AWS.Cryptography.MaterialProviders.ICryptographicMaterialsManager value)
+    {
+      return ToDafny_N3_aws__N12_cryptography__N17_materialProviders__S38_CryptographicMaterialsManagerReference(value);
+    }
     internal static AWS.Cryptography.MaterialProviders.IKeyring FromDafny_N3_aws__N12_cryptography__N17_materialProviders__S19_CreateKeyringOutput__M7_keyring(Dafny.Aws.Cryptography.MaterialProviders.Types.IKeyring value)
     {
       return FromDafny_N3_aws__N12_cryptography__N17_materialProviders__S16_KeyringReference(value);
@@ -2494,6 +2546,14 @@ namespace AWS.Cryptography.MaterialProviders
               "Custom implementations of Keyring must extend KeyringBase.");
       }
     }
+    internal static System.Collections.Generic.List<string> FromDafny_N3_aws__N12_cryptography__N17_materialProviders__S21_EncryptionContextKeys(Dafny.ISequence<Dafny.ISequence<byte>> value)
+    {
+      return new System.Collections.Generic.List<string>(value.Elements.Select(FromDafny_N3_aws__N12_cryptography__N17_materialProviders__S21_EncryptionContextKeys__M6_member));
+    }
+    internal static Dafny.ISequence<Dafny.ISequence<byte>> ToDafny_N3_aws__N12_cryptography__N17_materialProviders__S21_EncryptionContextKeys(System.Collections.Generic.List<string> value)
+    {
+      return Dafny.Sequence<Dafny.ISequence<byte>>.FromArray(value.Select(ToDafny_N3_aws__N12_cryptography__N17_materialProviders__S21_EncryptionContextKeys__M6_member).ToArray());
+    }
     internal static System.Collections.Generic.List<AWS.Cryptography.MaterialProviders.IKeyring> FromDafny_N3_aws__N12_cryptography__N17_materialProviders__S11_KeyringList(Dafny.ISequence<Dafny.Aws.Cryptography.MaterialProviders.Types.IKeyring> value)
     {
       return new System.Collections.Generic.List<AWS.Cryptography.MaterialProviders.IKeyring>(value.Elements.Select(FromDafny_N3_aws__N12_cryptography__N17_materialProviders__S11_KeyringList__M6_member));
@@ -2511,14 +2571,6 @@ namespace AWS.Cryptography.MaterialProviders
       return Dafny.Map<Dafny.ISequence<byte>, Dafny.ISequence<byte>>.FromCollection(value.Select(pair =>
          new Dafny.Pair<Dafny.ISequence<byte>, Dafny.ISequence<byte>>(ToDafny_N3_aws__N12_cryptography__N17_materialProviders__S17_EncryptionContext__M3_key(pair.Key), ToDafny_N3_aws__N12_cryptography__N17_materialProviders__S17_EncryptionContext__M5_value(pair.Value))
      ));
-    }
-    internal static System.Collections.Generic.List<string> FromDafny_N3_aws__N12_cryptography__N17_materialProviders__S21_EncryptionContextKeys(Dafny.ISequence<Dafny.ISequence<byte>> value)
-    {
-      return new System.Collections.Generic.List<string>(value.Elements.Select(FromDafny_N3_aws__N12_cryptography__N17_materialProviders__S21_EncryptionContextKeys__M6_member));
-    }
-    internal static Dafny.ISequence<Dafny.ISequence<byte>> ToDafny_N3_aws__N12_cryptography__N17_materialProviders__S21_EncryptionContextKeys(System.Collections.Generic.List<string> value)
-    {
-      return Dafny.Sequence<Dafny.ISequence<byte>>.FromArray(value.Select(ToDafny_N3_aws__N12_cryptography__N17_materialProviders__S21_EncryptionContextKeys__M6_member).ToArray());
     }
     internal static System.Collections.Generic.List<AWS.Cryptography.MaterialProviders.EncryptedDataKey> FromDafny_N3_aws__N12_cryptography__N17_materialProviders__S20_EncryptedDataKeyList(Dafny.ISequence<Dafny.Aws.Cryptography.MaterialProviders.Types._IEncryptedDataKey> value)
     {
@@ -2672,6 +2724,14 @@ namespace AWS.Cryptography.MaterialProviders
     {
       return ToDafny_N3_aws__N12_cryptography__N17_materialProviders__S8_KmsKeyId(value);
     }
+    internal static string FromDafny_N3_aws__N12_cryptography__N17_materialProviders__S21_EncryptionContextKeys__M6_member(Dafny.ISequence<byte> value)
+    {
+      return FromDafny_N3_aws__N12_cryptography__N17_materialProviders__S9_Utf8Bytes(value);
+    }
+    internal static Dafny.ISequence<byte> ToDafny_N3_aws__N12_cryptography__N17_materialProviders__S21_EncryptionContextKeys__M6_member(string value)
+    {
+      return ToDafny_N3_aws__N12_cryptography__N17_materialProviders__S9_Utf8Bytes(value);
+    }
     internal static AWS.Cryptography.MaterialProviders.IKeyring FromDafny_N3_aws__N12_cryptography__N17_materialProviders__S11_KeyringList__M6_member(Dafny.Aws.Cryptography.MaterialProviders.Types.IKeyring value)
     {
       return FromDafny_N3_aws__N12_cryptography__N17_materialProviders__S16_KeyringReference(value);
@@ -2693,14 +2753,6 @@ namespace AWS.Cryptography.MaterialProviders
       return FromDafny_N3_aws__N12_cryptography__N17_materialProviders__S9_Utf8Bytes(value);
     }
     internal static Dafny.ISequence<byte> ToDafny_N3_aws__N12_cryptography__N17_materialProviders__S17_EncryptionContext__M5_value(string value)
-    {
-      return ToDafny_N3_aws__N12_cryptography__N17_materialProviders__S9_Utf8Bytes(value);
-    }
-    internal static string FromDafny_N3_aws__N12_cryptography__N17_materialProviders__S21_EncryptionContextKeys__M6_member(Dafny.ISequence<byte> value)
-    {
-      return FromDafny_N3_aws__N12_cryptography__N17_materialProviders__S9_Utf8Bytes(value);
-    }
-    internal static Dafny.ISequence<byte> ToDafny_N3_aws__N12_cryptography__N17_materialProviders__S21_EncryptionContextKeys__M6_member(string value)
     {
       return ToDafny_N3_aws__N12_cryptography__N17_materialProviders__S9_Utf8Bytes(value);
     }
